Improve SimTactics.

theories/Equiv/SimII.v
@@ -1,6 +1,6 @@
 Require Import List paco2.
-Require Export Util Var Val Exp Env Map CSet AutoIndTac IL AllInRel.
-Require Export Sim SimTactics IL BlockType.
+Require Export Util Var Val Exp Env Map CSet AutoIndTac IL AllInRel Sawtooth.
+Require Export Sim SimTactics IL InRel.
 
 Set Implicit Arguments.
 Unset Printing Records.
@@ -15,6 +15,8 @@ Class ProofRelationI (A:Type) := {
     (* Relates environments according to analysis information *)
     IndexRelI : 〔A〕 -> nat -> nat -> Prop;
     Image : 〔A〕 -> nat;
+    ArgLengthMatchI : forall E E' a Z Z' VL VL',
+        ParamRelI a Z Z' -> ArgRelI E E' a VL VL' -> length Z = length VL /\ length Z' = length VL';
     IndexRelDrop : forall AL' AL n n', IndexRelI (AL' ++ AL) n n' ->
                                   n >= length AL'
                                   -> IndexRelI AL (n - length AL') (n' - Image AL')
@@ -25,7 +27,7 @@ Definition irel := rel3 simtype (fun _ : simtype => I.state)
 
 Coercion labN : lab >-> nat.
 
-Definition paramrel A (PR:ProofRelationI A)  AL L L' :=
+Definition paramrel A (PR:ProofRelationI A) AL L L' :=
   forall (f f':lab) Z s i Z' s' i' a,
     IndexRelI AL f f'
     -> get AL f a
@@ -41,10 +43,8 @@ Definition app_r t (r:irel) A (PR:ProofRelationI A) AL (L L':I.labenv) :=
     -> get L' f' (I.blockI Z' s' i')
     -> forall E E' Yv Y'v Y Y',
         ArgRelI E E' a Yv Y'v
-        -> omap (op_eval E) Y = Some Yv
-        -> omap (op_eval E') Y' = Some Y'v
-        -> ❬Z❭ = ❬Yv❭
-        -> ❬Z'❭ = ❬Y'v❭
+        -> omap (exp_eval E) Y = Some Yv
+        -> omap (exp_eval E') Y' = Some Y'v
         -> r t (L, E, stmtApp f Y)
             (L', E', stmtApp f' Y').
 
@@ -56,39 +56,20 @@ Proof.
   intros Lr LE; hnf; intros; eauto.
 Qed.
 
-Definition indexes_exists {A} (PR:ProofRelationI A) AL (L L' : I.labenv) :=
-  forall n n' a b, IndexRelI AL n n' -> get AL n a -> get L n b -> exists b', get L' n' b'.
-
-Definition indexwise_indexes_exists A (PR:ProofRelationI A) (F F':〔params * stmt〕) AL' AL :=
-  forall n n' Zs a,
-    IndexRelI (AL' ++ AL) n n'
-    -> get AL' n a
-    -> get F n Zs
-    -> exists Zs', get F' n' Zs'.
-
 Definition labenv_sim t (r:irel)
            {A} (PR:ProofRelationI A) (AL:list A) L L' :=
   length AL = length L /\
-  smaller L' /\
-  smaller L /\
+  sawtooth L' /\
+  sawtooth L /\
   paramrel PR AL L L' /\
-  indexes_exists PR AL L L' /\
   app_r t r PR AL L L'.
-
-Lemma labenv_sim_nil t r A PR
-  : @labenv_sim t r A PR nil nil nil.
-Proof.
-  do 5 (try split); hnf; intros; isabsurd.
-Qed.
-
-Hint Immediate labenv_sim_nil.
 
 Lemma labenv_sim_mon t (r r':irel) A (PR:ProofRelationI A) AL L L'
   :  labenv_sim t r PR AL L L'
     -> (forall t x y, r t x y -> r' t x y)
     -> labenv_sim t r' PR AL L L'.
 Proof.
-  intros [LEN [STL [STL' [PAR [IE SIM]]]]] LE; hnf; do 5 (try split); eauto.
+  intros [LEN [STL [STL' [PAR SIM]]]] LE; hnf; repeat split; eauto.
   eapply app_r_mon; eauto.
 Qed.
 
@@ -111,33 +92,24 @@ Proof.
   intros Idx LE; hnf; intros; eauto.
 Qed.
 
-
-Lemma bodies_r_app_r t A (PR:ProofRelationI A) AL L L' r
-  : bodies_r t r PR AL L L' L L'
-    -> app_r t (sim'r r) PR AL L L'.
-Proof.
-  intros SIM.
-  hnf; intros.
-  pone_step; simpl; eauto with len.
-Qed.
-
 Lemma fix_compatible_bodies t A (PR:ProofRelationI A) AL L L'
-  : (forall (r:irel) L1 L2, app_r t (sim'r r) PR AL L1 L2
+  : (forall r L1 L2, app_r t (sim'r r) PR AL L1 L2
           -> bodies_r t (sim'r r) PR AL L1 L2 L L')
+    -> paramrel PR AL L L'
     -> forall r, bodies_r t (sim'r r) PR AL L L' L L'.
 Proof.
-  intros ISIM r.
-  pcofix CIH;
-  change (bodies_r t (sim'r r) PR AL L L' L L');
-  change (bodies_r t r PR AL L L' L L') in CIH.
+  intros ISIM LP r. pcofix CIH.
   eapply ISIM.
-  eapply bodies_r_app_r; eauto.
+  hnf; intros.
+  exploit LP; eauto.
+  exploit ArgLengthMatchI; eauto; dcr.
+  pone_step; simpl; eauto with len.
 Qed.
 
 Lemma stepGoto_mapi L blk Y E vl f F k
       (Ldef:get L (counted f - ❬F❭) blk)
       (len:length (I.block_Z blk) = length Y)
-      (def:omap (op_eval E) Y = Some vl) E'
+      (def:omap (exp_eval E) Y = Some vl) E'
       (updOk:E [I.block_Z blk <-- List.map Some vl] = E')
       (ST:smaller L) (GE: counted f >= ❬F❭) (EQ:k = counted f - ❬F❭ - block_n blk)
   : I.step (mapi I.mkBlock F ++ L, E, stmtApp f Y) EvtTau
@@ -153,7 +125,7 @@ Proof.
   orewrite (counted f - ❬mapi I.mkBlock F❭ - block_n blk
             =  (counted f - block_n blk) - ❬mapi I.mkBlock F❭).
   rewrite <- (drop_app_gen _ (mapi I.mkBlock F)); eauto.
-  eapply I.StepGoto; eauto.
+  eapply I.stepGoto; eauto.
   rewrite get_app_ge. rewrite mapi_length. eauto. omega.
 Qed.
 
@@ -165,7 +137,6 @@ Definition indexwise_r t (r:irel) A (PR:ProofRelationI A) AL' F F' AL L L' :=
     -> get AL' n a
     -> forall E E' VL VL',
         ArgRelI E E' a VL VL'
-
         -> r t (L, E[Z <-- List.map Some VL], s)
             (L', E'[Z' <-- List.map Some VL'], s').
 
@@ -177,7 +148,7 @@ Proof.
   intros Idx LE; hnf; intros; eauto.
 Qed.
 
-Definition indexwise_paramrel A (PR:ProofRelationI A) (F F':〔params * stmt〕) AL' AL :=
+Definition indexwise_proofrel A (PR:ProofRelationI A) (F F':〔params * stmt〕) AL' AL :=
   forall n n' Z s Z' s' a,
     IndexRelI (AL' ++ AL) n n'
     -> get F n (Z,s)
@@ -185,19 +156,17 @@ Definition indexwise_paramrel A (PR:ProofRelationI A) (F F':〔params * stmt〕)
     -> get AL' n a
     -> ParamRelI a Z Z'.
 
-Definition separates A (PR:ProofRelationI A) AL' AL (F F':〔params * stmt〕) :=
-  length AL' = length F
-  /\ Image AL' = length F'
-  /\ (forall n n', IndexRelI (AL' ++ AL) n n' -> n < length F -> n' < length F')
-  /\  (forall n n', IndexRelI (AL' ++ AL) n n' -> n >= length F -> n' >= length F').
 
-Lemma complete_paramrel A (PR:ProofRelationI A) F F' AL' AL L L'
-  : indexwise_paramrel PR F F' AL' AL
+Lemma indexwise_paramrel A (PR:ProofRelationI A) F F' AL' AL L L'
+  : indexwise_proofrel PR F F' AL' AL
     -> paramrel PR AL L L'
-    -> separates PR AL' AL F F'
+    -> (forall n n', IndexRelI (AL' ++ AL) n n' -> n < length F -> n' < length F')
+    -> (forall n n', IndexRelI (AL' ++ AL) n n' -> n >= length F -> n' >= length F')
+    -> Image AL' = length F'
+    -> length AL' = length F
     -> paramrel PR (AL' ++ AL) (mapi I.mkBlock F ++ L) (mapi I.mkBlock F' ++ L').
 Proof.
-  intros IPR PAR [Len1 [Img [Ilt Ige]]].
+  intros IPR PAR Ilt Ige Img Len1.
   hnf; intros ? ? ? ? ? ? ? ? ? RN GetAL GetFL GetL'.
   eapply get_app_cases in GetFL; destruct GetFL as [GetFL'| [GetFL GE]].
   - exploit Ilt; eauto. eapply get_range in GetFL'.
@@ -214,39 +183,21 @@ Proof.
     rewrite Len1; eauto. rewrite Img; rewrite mapi_length in *; eauto.
 Qed.
 
-Lemma complete_indexes_exists A (PR:ProofRelationI A) F F' AL' AL L L'
-  : indexwise_indexes_exists PR F F' AL' AL
-    -> indexes_exists PR AL L L'
-    -> separates PR AL' AL F F'
-    -> indexes_exists PR (AL' ++ AL) (mapi I.mkBlock F ++ L) (mapi I.mkBlock F' ++ L').
-Proof.
-  intros IIE IE [Len1 [Img [Ilt Ige]]].
-  hnf; intros ? ? ? ? RN GetAL GetF.
-  assert (Len3:❬AL'❭ = ❬mapi I.mkBlock F❭) by eauto with len.
-  eapply get_app_cases in GetF. destruct GetF as [GetF| [GetFL GE]].
-  + inv_get. edestruct IIE; eauto.
-    eexists; eapply get_app, get_mapi; eauto.
-  + eapply get_app_right_ge in GetAL; [ | rewrite Len3; eauto ].
-    exploit Ige; eauto. rewrite mapi_length in *; eauto.
-    eapply IndexRelDrop in RN; [| rewrite Len3; eauto].
-    edestruct IE; eauto. rewrite Len3. eauto.
-    rewrite Img in H0. eexists.
-    eapply get_app_right; eauto. rewrite mapi_length in *. omega.
-Qed.
-
-Hint Unfold separates.
+Definition separates A (PR:ProofRelationI A) AL' AL (F F':〔params * stmt〕) :=
+  length AL' = length F
+  /\ Image AL' = length F'
+  /\ (forall n n', IndexRelI (AL' ++ AL) n n' -> n < length F -> n' < length F')
+  /\  (forall n n', IndexRelI (AL' ++ AL) n n' -> n >= length F -> n' >= length F').
 
 Lemma labenv_sim_extension' t r A (PR:ProofRelationI A) (AL AL':list A) F F' L L'
   : indexwise_r t (sim'r r \3/ r) PR AL' F F' AL (mapi I.mkBlock F ++ L) (mapi I.mkBlock F' ++ L')
-    -> indexwise_paramrel PR F F' AL' AL
-    -> indexwise_indexes_exists PR F F' AL' AL
+    -> indexwise_proofrel PR F F' AL' AL
     -> separates PR AL' AL F F'
     -> labenv_sim t (sim'r r) PR AL L L'
     -> labenv_sim t (sim'r r) PR (AL' ++ AL) (mapi I.mkBlock F ++ L) (mapi I.mkBlock F' ++ L').
 Proof.
-  intros SIM IPR IIE [Len2 [Img [Ilt Ige]]] [Len1 [STL [STL' [PAR [IE LSIM]]]]].
-  hnf; do 5 (try split);
-    eauto 20 using smaller_I_mkBlocks, complete_paramrel, complete_indexes_exists with len.
+  intros SIM IPR [Len2 [Img [Ilt Ige]]] [Len1 [STL [STL' [PAR LSIM]]]].
+  hnf; repeat split; eauto using sawtooth_I_mkBlocks, indexwise_paramrel with len.
   intros f f' ? ? ? ? ? ? ? RN GetAL GetFL GetL'.
   assert (Len3:❬AL'❭ = ❬mapi I.mkBlock F❭) by eauto with len.
   eapply get_app_cases in GetFL. destruct GetFL as [GetFL'| [GetFL GE]].
@@ -254,6 +205,8 @@ Proof.
     rewrite mapi_length in GetFL'; eauto.
     eapply get_app_lt_1 in GetL'; [| rewrite mapi_length; eauto ].
     inv_get. destruct x0 as [Z s], x as [Z' s']. simpl in *. clear EQ0 EQ.
+    exploit IPR; eauto.
+    exploit (ArgLengthMatchI); eauto; dcr.
     pone_step; simpl; eauto using get_app, get_mapi; simpl; eauto with len.
     orewrite (f-f=0). orewrite (f'-f'=0). simpl.
     exploit SIM; eauto.
@@ -264,28 +217,85 @@ Proof.
     eapply IndexRelDrop in RN; eauto; [| rewrite Len3; eauto].
     exploit (LSIM (LabI  (f - ❬AL'❭)) (LabI (f' - Image AL'))) as SIMR; eauto.
     rewrite Len3; eauto. rewrite Img; eauto.
+    exploit (PAR (LabI  (f - ❬AL'❭)) (LabI (f' - Image AL'))); eauto.
+    rewrite Len3; eauto. rewrite Img; eauto.
+    exploit (ArgLengthMatchI); eauto; dcr.
     eapply (@sim_Y_left I.state _ I.state _).
     eapply (@sim_Y_right I.state _ I.state _).
     rewrite Img in SIMR. rewrite Len3 in SIMR.
     eapply paco3_mon; [| eauto].
     eapply SIMR; eauto.
     econstructor; simpl; eauto with len. simpl. eauto with len.
-    eapply stepGoto_mapi; simpl in *; eauto with len.
+    eapply stepGoto_mapi; simpl in *; eauto using @sawtooth_smaller with len.
     econstructor; simpl; eauto. simpl. eauto with len.
-    eapply stepGoto_mapi; simpl in *; eauto with len.
+    eapply stepGoto_mapi; simpl in *; eauto using @sawtooth_smaller with len.
 Qed.
+
+(*
+Lemma labenv_sim_extension' t A (PR:ProofRelationI A) (AL AL':list A) F F' L L'
+  : (forall r L1 L2, labenv_sim t (sim'r r) PR (AL' ++ AL) L1 L2
+                -> indexwise_r t (sim'r r) PR AL' F F' AL L1 L2)
+    -> indexwise_proofrel PR F F' AL' AL
+    -> separates PR AL' AL F F'
+    -> paramrel PR AL L L'
+    -> sawtooth L
+    -> sawtooth L'
+    -> forall r, labenv_sim t (sim'r r) PR AL L L'
+        -> app_r t (sim'r r) PR (AL' ++ AL) (mapi I.mkBlock F ++ L) (mapi I.mkBlock F' ++ L').
+Proof.
+  intros SIM IPR [Len2 [Img [Ilt Ige]]] PAR STL STL' r LSIM. pcofix CIH.
+  intros f f' ? ? ? ? ? ? ? RN GetAL GetFL GetL'.
+  assert (Len1:❬AL'❭ = ❬mapi I.mkBlock F❭) by eauto with len.
+  eapply get_app_cases in GetFL. destruct GetFL as [GetFL'| [GetFL GE]].
+  - exploit Ilt; eauto. eapply get_range in GetFL'.
+    rewrite mapi_length in GetFL'; eauto.
+    eapply get_app_lt_1 in GetL'; [| rewrite mapi_length; eauto ].
+    inv_get. destruct x0 as [Z s], x as [Z' s']. simpl in *. clear EQ0 EQ.
+    exploit IPR; eauto.
+    exploit (ArgLengthMatchI); eauto; dcr.
+    exploit SIM.
+    repeat split; [ | | | | eapply app_r_mon; eauto];
+      eauto using sawtooth_I_mkBlocks, indexwise_paramrel with len.
+    hnf in LSIM; dcr; eauto with len.
+    exploit H1; eauto.
+    pone_step; simpl; eauto using get_app, get_mapi; simpl; eauto with len.
+    left.
+    orewrite (f-f=0). orewrite (f'-f'=0). simpl.
+    exploit H0; eauto.
+  - exploit Ige; eauto. rewrite mapi_length in GE; eauto.
+    eapply get_app_right_ge in GetAL; [ | rewrite Len1; eauto ].
+    eapply get_app_right_ge in GetL'; [ | rewrite mapi_length; eauto ].
+    rewrite mapi_length in *.
+    eapply IndexRelDrop in RN; eauto; [| rewrite Len1; eauto].
+    destruct LSIM as [Len3 [STLx [STL'x [PARx LSIM]]]].
+    exploit (LSIM (LabI  (f - ❬AL'❭)) (LabI (f' - Image AL'))) as SIMR; eauto.
+    rewrite Len1; eauto. rewrite Img; eauto.
+    exploit (PAR (LabI  (f - ❬AL'❭)) (LabI (f' - Image AL'))); eauto.
+    rewrite Len1; eauto. rewrite Img; eauto.
+    exploit (ArgLengthMatchI); eauto; dcr.
+    eapply (@sim_Y_left I.state _ I.state _).
+    eapply (@sim_Y_right I.state _ I.state _).
+    rewrite Img in SIMR. rewrite Len1 in SIMR.
+    eapply paco3_mon; [| eauto].
+    eapply SIMR; eauto.
+    econstructor; simpl; eauto with len. simpl. eauto with len.
+    eapply stepGoto_mapi; simpl in *; eauto using @sawtooth_smaller with len.
+    econstructor; simpl; eauto. simpl. eauto with len.
+    eapply stepGoto_mapi; simpl in *; eauto using @sawtooth_smaller with len.
+Qed.
+ *)
+
 
 Lemma fix_compatible_separate t A (PR:ProofRelationI A) AL' AL F F' L L'
   : (forall r,
         labenv_sim t (sim'r r) PR (AL' ++ AL) (mapi I.mkBlock F ++ L) (mapi I.mkBlock F' ++ L')
         -> indexwise_r t (sim'r r) PR AL' F F' AL (mapi I.mkBlock F ++ L) (mapi I.mkBlock F' ++ L'))
-    -> indexwise_paramrel PR F F' AL' AL
-    -> indexwise_indexes_exists PR F F' AL' AL
+    -> indexwise_proofrel PR F F' AL' AL
     -> separates PR AL' AL F F'
     -> forall r, labenv_sim t (sim'r r) PR AL L L'
            -> indexwise_r t (sim'r r) PR AL' F F' AL (mapi I.mkBlock F ++ L) (mapi I.mkBlock F' ++ L').
 Proof.
-  intros ISIM LP IE SEP r SIML. pcofix CIH.
+  intros ISIM LP SEP r SIML. pcofix CIH.
   eapply ISIM.
   eapply labenv_sim_extension'; eauto.
   eauto using indexwise_r_mon; eauto.
@@ -298,13 +308,12 @@ Lemma labenv_sim_extension t A (PR:ProofRelationI A) (AL AL':list A) F F' L L'
   : (forall r,
         labenv_sim t (sim'r r) PR (AL' ++ AL) (mapi I.mkBlock F ++ L) (mapi I.mkBlock F' ++ L')
         -> indexwise_r t (sim'r r) PR AL' F F' AL (mapi I.mkBlock F ++ L) (mapi I.mkBlock F' ++ L'))
-    -> indexwise_paramrel PR F F' AL' AL
-    -> indexwise_indexes_exists PR F F' AL' AL
+    -> indexwise_proofrel PR F F' AL' AL
     -> separates PR AL' AL F F'
     -> forall r, labenv_sim t (sim'r r) PR AL L L'
         -> labenv_sim t (sim'r r) PR (AL' ++ AL) (mapi I.mkBlock F ++ L) (mapi I.mkBlock F' ++ L').
 Proof.
-  intros ISIM IP IE SEP r SIML.
+  intros ISIM IP SEP r SIML.
   eapply labenv_sim_extension'; eauto.
   eapply indexwise_r_mon.
   eapply fix_compatible_separate; eauto. eauto.
@@ -319,45 +328,33 @@ Class PointwiseProofRelationI (A:Type) := {
        and closure environments *)
     ArgRelIP : onv val -> onv val -> A-> list val -> list val -> Prop;
     (* Relates environments according to analysis information *)
+    ArgLengthMatchIP : forall E E' a Z Z' VL VL',
+        ParamRelIP a Z Z' -> ArgRelIP E E' a VL VL' -> length Z = length VL /\ length Z' = length VL';
 }.
 
 Lemma pointwise_PR_as_PR A
   : PointwiseProofRelationI A -> ProofRelationI A.
 Proof.
-  intros. destruct X as [B C].
-  eapply (Build_ProofRelationI B C (fun L n n' => eq n n') (@length _)).
-  - intros; dcr; subst; eauto.
+  intros. destruct X as [B C D].
+  eapply (Build_ProofRelationI B C (fun _ => eq) (@length _) D).
+  intros; eauto.
 Defined.
 
 Hint Resolve pointwise_PR_as_PR : typeclass_instances.
+
 Coercion pointwise_PR_as_PR : PointwiseProofRelationI >-> ProofRelationI.
 
-Lemma IndexRelIP_eq A PR L n n'
-  : @IndexRelI A (pointwise_PR_as_PR PR) L n n' <-> n = n'.
-Proof.
-  destruct PR; simpl. reflexivity.
-Qed.
-
-Lemma IndexRelIP_refl A PR L n
-  : @IndexRelI A (pointwise_PR_as_PR PR) L n n.
-Proof.
-  destruct PR; simpl. reflexivity.
-Qed.
-
-Hint Resolve IndexRelIP_refl.
 
 Lemma labenv_sim_extension_ptw t A (PR:PointwiseProofRelationI A) (AL AL':list A) F F' L L'
-  : (forall r ,
-        labenv_sim t (sim'r r) PR (AL' ++ AL) (mapi I.mkBlock F ++ L) (mapi I.mkBlock F' ++ L')
-        -> indexwise_r t (sim'r r) PR AL' F F' AL (mapi I.mkBlock F ++ L) (mapi I.mkBlock F' ++ L'))
-    -> indexwise_paramrel PR F F' AL' AL
-    -> indexwise_indexes_exists PR F F' AL' AL
+  : (forall r L1 L2, labenv_sim t (sim'r r) PR (AL' ++ AL) L1 L2
+                -> indexwise_r t (sim'r r) PR AL' F F' AL L1 L2)
+    -> indexwise_proofrel PR F F' AL' AL
     -> length AL' = length F
     -> length F = length F'
     -> forall r, labenv_sim t (sim'r r) PR AL L L'
         -> labenv_sim t (sim'r r) PR (AL' ++ AL) (mapi I.mkBlock F ++ L) (mapi I.mkBlock F' ++ L').
 Proof.
-  intros ISIM IP IE Len1 Len2 r SIML.
+  intros ISIM IP Len1 Len2 r SIML.
   assert (separates PR AL' AL F F'). {
     destruct SIML; dcr.
     hnf; destruct PR; simpl; repeat split; intros; omega.
@@ -365,39 +362,4 @@ Proof.
   eapply labenv_sim_extension'; eauto.
   eapply indexwise_r_mon.
   eapply fix_compatible_separate; eauto. eauto.
-Qed.
-
-Lemma labenv_sim_app i A (PR:ProofRelationI A) AL L L' r V V' Y Y' (f f':lab) a
-  : labenv_sim i (sim'r r) PR AL L L'
-    -> get AL f a
-    -> IndexRelI AL f f'
-    -> (forall Z s n Z' s' n',
-         get L f (I.blockI Z s n)
-         -> get L' f' (I.blockI Z' s' n')
-         -> ParamRelI a Z Z'
-         -> (forall Yv, omap (op_eval V) Y = ⎣ Yv ⎦ -> ❬Z❭ = ❬Yv❭
-                 -> exists Y'v, omap (op_eval V') Y' = ⎣ Y'v ⎦ /\
-                          ❬Z'❭ = ❬Y'v❭ /\ ArgRelI V V' a Yv Y'v)
-           /\ (if isBisim i then
-                (omap (op_eval V) Y = None -> omap (op_eval V') Y' = None)
-                /\ (❬Z❭ <> ❬Y❭ -> ❬Z'❭ <> ❬Y'❭)
-              else True))
-    -> sim'r r i (L, V, stmtApp f Y) (L', V', stmtApp f' Y').
-Proof.
-  intros LSIM GetAL RN ALL.
-  edestruct LSIM as [Len1 [STL [STL' [PAR [IE SIM]]]]]; eauto; dcr.
-  inv_get. edestruct IE; eauto.
-  destruct x as [Z s n], x0 as [Z' s' n'].
-  exploit PAR; eauto.
-  edestruct ALL as [A1 A2]; eauto; dcr.
-  case_eq (omap (op_eval V) Y); intros.
-  - decide (❬Z❭ = ❬Y❭).
-    + edestruct A1; dcr; eauto with len.
-    + destruct i; simpl in *; dcr.
-      * exploit H4; eauto.
-        pno_step.
-      * perr.
-  - destruct i; simpl in *; dcr.
-    + exploit H3; eauto. pno_step.
-    + perr.
 Qed.
