theories/Equiv/SimA.v
@@ -1,0 +1,337 @@
+Require Import Util Option AllInRel Sawtooth Get.
+Require Export SmallStepRelations StateType.
+
+Set Implicit Arguments.
+Unset Printing Records.
+
+(** * Simulation *)
+(** A characterization of simulation equivalence on states;
+works only for internally deterministic semantics *)
+
+Inductive simtype := Bisim | Sim.
+
+CoInductive sim {S} `{StateType S} {S'} `{StateType S'}  : simtype -> S -> S' -> Prop :=
+  | simSilent t (σ1 σ1':S) (σ2 σ2':S') : (* result σ1 = result σ2 -> *)
+      plus2 step σ1 nil σ1'
+      -> plus2 step σ2 nil σ2'
+      -> sim t σ1' σ2'
+      -> sim t σ1 σ2
+  | simExtern t (pσ1 σ1:S) (pσ2 σ2:S') : (* result σ1 = result σ2 -> *)
+      star2 step pσ1 nil σ1
+      -> star2 step pσ2 nil σ2
+      -> activated σ1
+      -> activated σ2
+      -> (forall evt σ1', step σ1 evt σ1' -> exists σ2', step σ2 evt σ2' /\ sim t σ1' σ2')
+      -> (forall evt σ2', step σ2 evt σ2' -> exists σ1', step σ1 evt σ1' /\ sim t σ1' σ2')
+      -> sim t pσ1 pσ2
+  | simErr (σ1 σ1':S) (σ2:S')
+    : result σ1' = None
+      -> star2 step σ1 nil σ1'
+      -> normal2 step σ1'
+      -> sim Sim σ1 σ2
+  | simTerm t (σ1 σ1':S) (σ2 σ2':S')
+    : result σ1' = result σ2'
+      -> star2 step σ1 nil σ1'
+      -> star2 step σ2 nil σ2'
+      -> normal2 step σ1'
+      -> normal2 step σ2'
+      -> sim t σ1 σ2.
+
+Arguments sim [S] {H} [S'] {H0} _ _ _.
+
+Lemma sim_refl {S} `{StateType S} t (σ:S)
+      : sim t σ σ.
+Proof.
+  revert σ. cofix.
+  intros. destruct (step_dec σ) as [[[] []]|].
+  - eapply simExtern; intros; eauto using star2_refl; eexists; eauto.
+  - eapply simSilent; eauto using plus2O.
+  - eapply simTerm; eauto using star2_refl.
+Qed.
+
+Inductive sim_gen {S} `{StateType S} {S'} `{StateType S'}
+          (r: simtype -> S -> S' -> Prop)  : simtype -> S -> S' -> Prop :=
+  | sim'Silent t (σ1 σ1':S) (σ2 σ2':S') : (* result σ1 = result σ2 -> *)
+      plus2 step σ1 nil σ1'
+      -> plus2 step σ2 nil σ2'
+      -> r t σ1' σ2'
+      -> sim_gen r t σ1 σ2
+  | sim'Extern t (pσ1 σ1:S) (pσ2 σ2:S') : (* result σ1 = result σ2 -> *)
+      star2 step pσ1 nil σ1
+      -> star2 step pσ2 nil σ2
+      -> activated σ1
+      -> activated σ2
+      -> (forall evt σ1', step σ1 evt σ1' -> exists σ2', step σ2 evt σ2' /\ r t σ1' σ2')
+      -> (forall evt σ2', step σ2 evt σ2' -> exists σ1', step σ1 evt σ1' /\ r t σ1' σ2')
+      -> sim_gen r t pσ1 pσ2
+  | sim'Err (σ1 σ1':S) (σ2:S')
+    : result σ1' = None
+      -> star2 step σ1 nil σ1'
+      -> normal2 step σ1'
+      -> sim_gen r Sim σ1 σ2
+  | sim'Term t (σ1 σ1':S) (σ2 σ2':S')
+    : result σ1' = result σ2'
+      -> star2 step σ1 nil σ1'
+      -> star2 step σ2 nil σ2'
+      -> normal2 step σ1'
+      -> normal2 step σ2'
+      -> sim_gen r t σ1 σ2.
+
+Arguments sim_gen [S] {H} [S'] {H0} r _ _ _.
+
+Hint Constructors sim_gen.
+
+
+Definition rel2 T0 T1 :=
+  forall (x0: T0) (x1: T1 x0), Prop.
+Implicit Arguments rel2 [].
+
+Definition pacoid {A : Type} (a: A) : A := a.
+
+Notation bot2 :=
+  (pacoid(fun _ _ => False)).
+
+Notation "p \2/ q" :=
+  (fun x0 x1 => p x0 x1 \/ q x0 x1)
+  (at level 50, no associativity).
+
+Notation "p <_paco_2= q" :=
+  (forall _paco_x0 _paco_x1 (PR: p _paco_x0 _paco_x1 : Prop), q _paco_x0 _paco_x1 : Prop)
+  (at level 50, no associativity).
+
+Notation "p <2= q" :=
+  (forall x0 x1 (PR: p x0 x1 : Prop), q x0 x1 : Prop)
+  (at level 50, no associativity).
+
+Section Arg2_def.
+Variable T0 : Type.
+Variable T1 : forall (x0: @T0), Type.
+Variable gf : rel2 T0 T1 -> rel2 T0 T1.
+Implicit Arguments gf [].
+
+CoInductive paco2( r: rel2 T0 T1) x0 x1 : Prop :=
+| paco2_pfold pco
+    (LE : pco <2= (paco2 r \2/ r))
+    (SIM: gf pco x0 x1)
+.
+End Arg2_def.
+Implicit Arguments paco2 [ T0 T1 ].
+
+Section Arg2_1.
+
+Definition monotone2 T0 T1 (gf: rel2 T0 T1 -> rel2 T0 T1) :=
+  forall x0 x1 r r' (IN: gf r x0 x1) (LE: r <2= r'), gf r' x0 x1.
+
+Variable T0 : Type.
+Variable T1 : forall (x0: @T0), Type.
+Variable gf : rel2 T0 T1 -> rel2 T0 T1.
+
+Theorem paco2_acc: forall
+  l r (OBG: forall rr (INC: r <2= rr) (CIH: l <_paco_2= rr), l <_paco_2= paco2 gf rr),
+  l <2= paco2 gf r.
+Proof.
+  intros; assert (SIM: paco2 gf (r \2/ l) x0 x1) by eauto.
+  clear PR. revert x0 x1 SIM. cofix; intros.
+  destruct SIM.
+  econstructor; [ | eapply SIM].
+  intros. exploit LE; eauto.
+  destruct H. left. eapply paco2_acc. eauto.
+  destruct H. right; eauto.
+  left. eapply paco2_acc.
+  eapply OBG; eauto.
+Qed.
+
+Theorem paco2_mon: monotone2 (paco2 gf).
+Proof.
+  hnf. cofix CIH; intros.
+  destruct IN. econstructor; [ | eapply SIM].
+  intros. edestruct LE0; eauto.
+Qed.
+
+Theorem paco2_mult_strong: forall r,
+  paco2 gf (paco2 gf r \2/ r) <2= paco2 gf r.
+Proof.
+  cofix CIH; intros.
+  destruct PR. econstructor; [ | eapply SIM].
+  intros. edestruct LE; eauto.
+Qed.
+
+Corollary paco2_mult: forall r,
+  paco2 gf (paco2 gf r) <2= paco2 gf r.
+Proof.
+  intros; eapply paco2_mult_strong, paco2_mon; eauto.
+Qed.
+
+Theorem paco2_fold: forall r,
+  gf (paco2 gf r \2/ r) <2= paco2 gf r.
+Proof. intros; econstructor; [ |eauto]; eauto. Qed.
+
+Theorem paco2_unfold: forall (MON: monotone2 gf) r,
+  paco2 gf r <2= gf (paco2 gf r \2/ r).
+Proof. unfold monotone2; intros; destruct PR; eauto. Qed.
+
+End Arg2_1.
+
+Hint Unfold monotone2.
+Hint Resolve paco2_fold.
+
+Arguments paco2_acc [T0 T1] gf l r OBG x0 x1 PR .
+Arguments paco2_mon [T0 T1] gf x0 x1 r r' IN LE.
+Arguments paco2_mult_strong [T0 T1] gf r x0 x1 PR.
+Arguments paco2_mult  [T0 T1] gf r x0 x1 PR.
+Arguments paco2_fold           [ T0 T1 ] gf r x0 x1 PR.
+Arguments paco2_unfold         [ T0 T1 ] gf MON r x0 x1 PR.
+
+
+Definition rel3 T0 T1 T2 :=
+  forall (x0: T0) (x1: T1 x0) (x2: T2 x0 x1), Prop.
+Arguments rel3 : clear implicits.
+
+Notation bot3 := (fun _ _ _ => False).
+
+Notation "p \3/ q" :=
+  (fun x0 x1 x2 => p x0 x1 x2 \/ q x0 x1 x2)
+  (at level 50, no associativity).
+
+Notation "p <3= q" :=
+  (forall x0 x1 x2 (P: p x0 x1 x2 : Prop), q x0 x1 x2 : Prop)
+  (at level 50, no associativity).
+
+Section Arg3_def.
+Variable T0 : Type.
+Variable T1 : forall (x0: T0), Type.
+Variable T2 : forall (x0: T0) (x1:T1 x0), Type.
+Variable gf : rel3 T0 T1 T2 -> rel3 T0 T1 T2.
+Implicit Arguments gf [].
+
+CoInductive paco3 (r: rel3 T0 T1 T2) x0 x1 x2 : Prop :=
+| paco3_pfold pco
+    (LE : pco <3= (paco3 r \3/ r))
+    (SIM: gf pco x0 x1 x2)
+.
+End Arg3_def.
+Arguments paco3 [ T0 T1 T2] gf r x0 x1 x2.
+
+Section Arg3_1.
+
+Definition monotone3 T0 T1 T2 (gf: rel3 T0 T1 T2 -> rel3 T0 T1 T2) :=
+  forall x0 x1 x2 r r' (IN: gf r x0 x1 x2) (LE: r <3= r'), gf r' x0 x1 x2.
+
+Variable T0 : Type.
+Variable T1 : forall (x0: T0), Type.
+Variable T2 : forall (x0: T0) (x1:T1 x0), Type.
+Variable gf : rel3 T0 T1 T2 -> rel3 T0 T1 T2.
+
+Theorem paco3_acc: forall
+    l r
+    (OBG: forall rr (INC: r <3= rr) (CIH: l <3= rr), l <3= paco3 gf rr),
+  l <3= paco3 gf r.
+Proof.
+  intros; assert (SIM: paco3 gf (r \3/ l) x0 x1 x2) by eauto.
+  clear P. revert x0 x1 x2 SIM. cofix; intros.
+  destruct SIM.
+  econstructor; [ | eapply SIM].
+  intros. edestruct LE as [? | [?|?]]; eauto.
+  - left. eapply paco3_acc.
+    eapply OBG; eauto.
+Qed.
+
+Theorem paco3_mon: monotone3 (paco3 gf).
+Proof.
+  hnf. cofix CIH; intros.
+  destruct IN. econstructor; [ | eapply SIM].
+  intros. edestruct LE0; eauto.
+Qed.
+
+Theorem paco3_mult_strong: forall r,
+  paco3 gf (paco3 gf r \3/ r) <3= paco3 gf r.
+Proof.
+  cofix CIH; intros.
+  destruct P. econstructor; [ | eapply SIM].
+  intros. edestruct LE; eauto.
+Qed.
+
+Corollary paco3_mult: forall r,
+  paco3 gf (paco3 gf r) <3= paco3 gf r.
+Proof.
+  intros; eapply paco3_mult_strong, paco3_mon; eauto.
+Qed.
+
+Theorem paco3_fold: forall r,
+  gf (paco3 gf r \3/ r) <3= paco3 gf r.
+Proof. intros; econstructor; [ |eauto]; eauto. Qed.
+
+Theorem paco3_unfold: forall (MON: monotone3 gf) r,
+  paco3 gf r <3= gf (paco3 gf r \3/ r).
+Proof. unfold monotone3; intros. destruct P; eauto. Qed.
+
+End Arg3_1.
+
+Hint Unfold monotone3.
+Hint Resolve paco3_fold.
+
+Arguments paco3_acc [T0 T1 T2] gf l r OBG x0 x1 x2 P.
+Arguments paco3_mon [T0 T1 T2] gf x0 x1 x2 r r' IN LE.
+Arguments paco3_mult_strong [T0 T1 T2] gf r x0 x1 x2 P.
+Arguments paco3_mult [T0 T1 T2] gf r x0 x1 x2 P.
+Arguments paco3_fold [ T0 T1 T2] gf r x0 x1 x2 P.
+Arguments paco3_unfold [ T0 T1 T2] gf MON r x0 x1 x2 P.
+
+
+
+
+Definition sim' t {S} `{StateType S} {S'} `{StateType S'} (σ1:S) (σ2:S')
+  := paco3 (@sim_gen S _ S' _) bot3 t σ1 σ2.
+Hint Unfold sim'.
+
+Definition sim'r {S} `{StateType S} {S'} `{StateType S'} r t (σ1:S) (σ2:S')
+  := paco3 (@sim_gen S _ S' _) r t σ1 σ2.
+Hint Unfold sim'r.
+
+Lemma sim_gen_mon {S} `{StateType S} {S'} `{StateType S'}
+: monotone3 (@sim_gen S _ S' _).
+Proof.
+  hnf; intros. inv IN; eauto using @sim_gen.
+  - econstructor 2; eauto; intros.
+    edestruct H5; eauto; dcr. eexists; eauto.
+    edestruct H6; eauto; dcr. eexists; eauto.
+Qed.
+
+Arguments sim_gen_mon [S] {H} [S'] {H0} [x0] [x1] [x2] r r' IN LE.
+
+Hint Resolve sim_gen_mon : paco.
+
+Lemma sim_sim' {S} `{StateType S} {S'} `{StateType S'} t (σ1:S) (σ2:S')
+: sim t σ1 σ2 -> sim' t σ1 σ2.
+Proof.
+  revert σ1 σ2. intros. eapply paco3_acc; [ | eapply H1]; intros.
+  intros. econstructor. eauto.
+  inv H2; eauto using sim_gen.
+  - econstructor 2; eauto; intros.
+    + edestruct H6; eauto; dcr. eexists; eauto.
+    + edestruct H7; eauto; dcr. eexists; eauto.
+Qed.
+
+
+Lemma sim'_sim {S} `{StateType S} {S'} `{StateType S'} t (σ1:S) (σ2:S')
+: sim' t σ1 σ2 -> sim t σ1 σ2.
+Proof.
+  revert t σ1 σ2. cofix CIH.
+  intros.
+  assert (sim_gen (paco3 (@sim_gen S _ S' _) bot3 \3/ bot3) t σ1 σ2).
+  punfold H1.
+  destruct H2. destruct H4.
+  - econstructor; eauto.
+  - exfalso; intuition.
+  - econstructor 2; eauto; intros.
+    + edestruct H6; eauto; dcr. destruct H11. eexists; eauto. exfalso; intuition.
+    + edestruct H7; eauto; dcr. destruct H11. eexists; eauto. exfalso; intuition.
+  - econstructor 3; eauto.
+  - econstructor 4; eauto.
+Qed.
+
+Lemma sim'_refl {S} `{StateType S} (σ:S) t
+      : sim' t σ σ.
+Proof.
+  eapply sim_sim'. eapply sim_refl.
+Qed.
