theories/Equiv/SimTactics.v
@@ -1,4 +1,5 @@
 Require Import Sim IL paco3.
+Require Export ILStateType.
 
 Ltac one_step := eapply simSilent; [ eapply plus2O; single_step
                               | eapply plus2O; single_step
@@ -66,18 +67,35 @@ Ltac pno_step_left :=
   pfold; econstructor 3; [ | eapply star2_refl|]; [ reflexivity | ]; stuck2.
 
 
-Lemma sim_let_op i r L L' V V' x x' e e' s s'
+Ltac perr :=
+  pfold; eapply sim'Err;
+  [ | eapply star2_refl | ];
+  [ repeat get_functional; try reflexivity
+  | repeat get_functional; stuck2 ].
+
+Set Implicit Arguments.
+
+Lemma sim_let_op X (IST:ILStateType X) i r (L L':X) V V' x x' e e' s s'
       (EQ:op_eval V e = op_eval V' e')
       (SIM: forall v, op_eval V e = Some v
                  -> (sim'r r \3/ r) i (L, V [x <- ⎣ v ⎦], s) (L', V' [x' <- ⎣ v ⎦], s'))
   : sim'r r i (L, V, stmtLet x (Operation e) s) (L', V', stmtLet x' (Operation e') s').
 Proof.
   case_eq (op_eval V e); intros.
-  * pone_step; eauto. rewrite EQ in H; eauto.
-  * pno_step.
+  * pfold; eapply sim'Silent; [ eapply plus2O
+                              | eapply plus2O
+                              | ].
+    eapply step_let_op; eauto. eauto.
+    eapply step_let_op. rewrite <- EQ. eauto. eauto.
+    eapply SIM; eauto.
+  * pfold. eapply sim'Term; [| eapply star2_refl | eapply star2_refl | | ];
+             [ simpl | | ].
+    rewrite !let_result; eauto.
+    eapply let_op_normal; eauto.
+    eapply let_op_normal; rewrite <- EQ; eauto.
 Qed.
 
-Lemma sim_let_call i r L L' V V' x x' f Y Y' s s'
+Lemma sim_let_call X (IST:ILStateType X) i r (L L':X) V V' x x' f Y Y' s s'
       (EQ: omap (op_eval V) Y = omap (op_eval V') Y')
       (SIM: forall v, (sim'r r \3/ r) i (L, V [x <- ⎣ v ⎦], s) (L', V' [x' <- ⎣ v ⎦], s'))
   : sim'r r i (L, V, stmtLet x (Call f Y) s) (L', V', stmtLet x' (Call f Y') s').
@@ -86,16 +104,15 @@ Proof.
   * pose proof H as H'. rewrite EQ in H'.
     pfold; eapply sim'Extern;
       [ eapply star2_refl
-      | eapply star2_refl | step_activated | step_activated | |].
-    intros ? ? STEP; inv STEP; eexists; split; [econstructor; eauto | ].
-    rewrite <- EQ. eauto. eapply SIM.
-    intros ? ? STEP; inv STEP; eexists; split; [econstructor; eauto | ].
-    rewrite EQ. eauto. eapply SIM.
-  * pno_step.
+      | eapply star2_refl
+      | step_activated; eauto using step_let_call
+      | step_activated; eauto using step_let_call | |];
+      intros ? ? STEP; eapply let_call_inversion in STEP; dcr; subst; eexists; split; try eapply step_let_call; eauto.
+    rewrite <- EQ; eauto.
+    rewrite EQ; eauto.
+  * pfold. eapply sim'Term; [| eapply star2_refl | eapply star2_refl | | ];
+             [ simpl | | ].
+    rewrite !let_result; eauto.
+    eapply let_call_normal; eauto.
+    eapply let_call_normal; rewrite <- EQ; eauto.
 Qed.
-
-Ltac perr :=
-  pfold; eapply sim'Err;
-  [ | eapply star2_refl | ];
-  [ repeat get_functional; try reflexivity
-  | repeat get_functional; stuck2 ].
