theories/IL/ILStateType.v
@@ -1,0 +1,49 @@
+Require Import IL.
+
+
+Class ILStateType X :=
+  {
+    statetype :> StateType (X * onv val * stmt);
+    step_let_op :  forall L E x e b v (def:op_eval E e = Some v),
+        step (L, E, stmtLet x (Operation e) b) EvtTau (L, E[x<-Some v], b);
+    step_let_call : forall L E x f Y s vl v (def:omap (op_eval E) Y = Some vl),
+        step  (L, E, stmtLet x (Call f Y) s) (EvtExtern (ExternI f vl v)) (L, E[x <- Some v], s);
+    let_op_normal :  forall L E x e b (def:op_eval E e = None),
+        normal2 step (L, E, stmtLet x (Operation e) b);
+    let_call_normal :  forall L E x f Y s (def:omap (op_eval E) Y = None),
+        normal2 step (L, E, stmtLet x (Call f Y) s);
+    let_call_inversion : forall L E x f Y s evt σ,
+        step  (L, E, stmtLet x (Call f Y) s) evt σ
+        -> exists vl v, omap (op_eval E) Y = Some vl
+                /\ evt = (EvtExtern (ExternI f vl v))
+                /\ σ = (L, E[x <- Some v], s);
+    let_result : forall L E x e s, result (L, E, stmtLet x e s) = None
+  }.
+
+
+Instance il_statetype_F : ILStateType F.labenv :=
+  {
+    statetype := statetype_F;
+    step_let_op := F.StepLet;
+    step_let_call := F.StepExtern
+  }.
+Proof.
+  - intros. stuck2.
+  - intros. stuck2.
+  - intros; inv H; eauto.
+  - intros; simpl; eauto.
+
+Defined.
+
+Instance il_statetype_I : ILStateType I.labenv :=
+  {
+    statetype := statetype_I;
+    step_let_op := I.StepLet;
+    step_let_call := I.StepExtern
+  }.
+Proof.
+  - intros. stuck2.
+  - intros. stuck2.
+  - intros; inv H; eauto.
+  - intros; simpl; eauto.
+Defined.
